EvmCompiler.lean
@@ -1,2 +1,2 @@
 import EvmCompiler.Assembly
-
+import EvmCompiler.Structured
